mark-and-sweep/spec/GC.Spec.ChunkedSweepCoalesce.Defs.fst
@@ -194,6 +194,14 @@ let chunked_is_infix (mh: MH.major_heap) (obj: obj_addr)
   : GTot bool
   = chunked_tag_of_object mh obj = Obj.infix_tag
 
+let chunked_is_infix_step
+    (mh: MH.major_heap)
+    (obj: obj_addr)
+  : Lemma
+      (chunked_is_infix mh obj ==
+       (chunked_tag_of_object mh obj = Obj.infix_tag))
+  = ()
+
 let chunked_set_object_color
     (mh: MH.major_heap) (obj: obj_addr) (color: Header.color_sem)
   : GTot MH.major_heap
